\documentclass{article}
\usepackage[utf8]{inputenc}
\usepackage[english]{babel}
\usepackage[a4paper,top=3.5cm,bottom=3.5cm,left=3.5cm,right=3.5cm,%
bindingoffset=0mm]{geometry}
\usepackage{amssymb}
\usepackage{amsmath}
\newtheorem{prop}{Proposition}
\newtheorem{lemma}{Lemma}
\newenvironment{proof}[1][Proof]{\begin{trivlist}
		\item[\hskip \labelsep {\bfseries #1}]}{\end{trivlist}}
\newcommand{\qed}{\nobreak \ifvmode \relax \else
	\ifdim\lastskip<1.5em \hskip-\lastskip
	\hskip1.5em plus0em minus0.5em \fi \nobreak
	\vrule height0.75em width0.75em depth0em\fi}
\usepackage{tikz}
\usepackage{graphicx}
\usepackage{rotating}
\usepackage{float}
\linespread{1.3}
\raggedbottom




%
\font\reali=msbm10 at 12pt
% subsets of real numbers
\newcommand{\real}{\hbox{\reali R}}
\newcommand{\realp}{\hbox{\reali R}_{\scriptscriptstyle +}}
\newcommand{\realpp}{\hbox{\reali R}_{\scriptscriptstyle ++}}
\newcommand{\R}{\mathbb{R}}
\DeclareMathOperator{\E}{\mathbb{E}}
%

\title{Stationarized System with Spillover}
\author{Marco Brianti\\Laura Gati}
\date{April 2018}

\begin{document}
	
	\maketitle

\Large{
	

\begin{equation}\label{eq:prodfuncfinal}
y_{c,t} = \Gamma_{c,t} k_{i,t}^{\gamma} h_{1,t}^{1 - a- b} k_{c,1,t}^a k_{i,1,t}^b
\end{equation}
\begin{equation}\label{eq:prodfuncinter}
y_{i,t} = \Gamma_{i,t} k_{i,t}^{\gamma} h_{2,t}^{1 - a- b} k_{c,2,t}^a k_{i,2,t}^b
\end{equation}
\begin{equation}\label{eq:LOMfinal}
k_{c,t+1} \exp{(g_c)} = (1 - \delta_c)k_{c,t} + i_{c,t}
\end{equation}
\begin{equation}\label{eq:LOMinter}
k_{i,t+1} \exp{(g_i)} = (1 - \delta_i)k_{i,t} + i_{i,t}
\end{equation}
\begin{equation}\label{eq:resourcefinal}
y_{c,t} = c_{t} + i_{c,t}
\end{equation}
\begin{equation}\label{eq:resourceinter}
y_{i,t} = i_{i,t}
\end{equation}
\begin{equation}\label{eq:intratEE}
w_{t} = \chi c_{t}
\end{equation}
\begin{equation}\label{eq:hardKconstr}
k_{c,t} = k_{c,1,t} + k_{c,2,t}
\end{equation}
\begin{equation}\label{eq:softKconstr}
k_{i,t} = k_{i,1,t} + k_{i,2,t}
\end{equation}
\begin{equation}\label{eq:hoursconstr}
h_{t} = h_{1,t} + h_{2,t}
\end{equation}
\begin{equation}\label{eq:intertEEhard}
1 = \beta \E \bigg[ (\exp{(g_c)})^{-1} \frac{c_{t}}{c_{t+1}} \bigg( r_{c,t+1} + 1 - \delta_c   \bigg)     \bigg]
\end{equation}
\begin{equation}\label{eq:intertEEsoft}
1 = \beta \E \bigg[ (\exp{(g_i)})^{-1} \frac{c_{t}}{c_{t+1}} \bigg( \frac{r_{i,t+1}}{p_t} + 1 - \delta_i  \bigg)     \bigg]
\end{equation}
\begin{equation}\label{eq:FOClaborfinal}
w_t = (1 - a - b)\Gamma_{c,t} k_{i,t}^{\gamma} h_{1,t}^{- a- b} k_{c,1,t}^a k_{i,1,t}^b
\end{equation}
\begin{equation}\label{eq:FOChardKfinal}
r_{c,t} = a \Gamma_{c,t} k_{i,t}^{\gamma} h_{1,t}^{1 - a- b} k_{c,1,t}^{a-1} k_{i,1,t}^b
\end{equation}
\begin{equation}\label{eq:FOCsoftKfinal}
r_{i,t} = b \Gamma_{c,t} k_{i,t}^{\gamma} h_{1,t}^{1 - a- b} k_{c,1,t}^a k_{i,1,t}^{b-1}
\end{equation}
\begin{equation}\label{eq:FOClaborinter}
\frac{w_t}{p_t} = (1 - a - b)\Gamma_{i,t} k_{i,t}^{\gamma} h_{2,t}^{- a- b} k_{c,2,t}^a k_{i,2,t}^b
\end{equation}
\begin{equation}\label{eq:FOChardKinter}
\frac{r_{c,t}}{p_t} = a \Gamma_{i,t} k_{i,t}^{\gamma} h_{2,t}^{1 - a- b} k_{c,2,t}^{a-1} k_{i,2,t}^b\\\
\end{equation}
\begin{equation}\label{eq:FOCsoftKinter}
\frac{r_{i,t}}{p_t} = b \Gamma_{i,t} k_{i,t}^{\gamma} h_{2,t}^{1 - a- b} k_{c,2,t}^a k_{i,2,t}^{b-1}
\end{equation}

\section*{Steady-State Procedure}

\subsection*{Step 0}

Divide \ref{eq:FOClaborfinal} over \ref{eq:FOClaborinter} and obtain
\begin{equation}\label{Pclosedform}
p = \frac{\Gamma_c}{\Gamma_i}.
\end{equation}
Solve for $r_c$ in \ref{eq:intertEEhard} and obtain
\begin{equation}
r_c = 1/\beta \exp(g_c) - (1-\delta_c)
\end{equation}
where $\exp(g_c) = \Gamma_c^{\frac{1-b-\gamma}{1-a-b-\gamma}} \Gamma_i^{\frac{b+\gamma}{1-a-b-\gamma}}$.
}

Solve for $r_i$ in \ref{eq:intertEEsoft} and obtain
\begin{equation}
r_i = 1/\beta \exp(g_i) - (1-\delta_i)
\end{equation}
where $\exp(g_i) = \Gamma_c^{\frac{a}{1-a-b-\gamma}} \Gamma_i^{\frac{1-a}{1-a-b-\gamma}}$.

\subsection*{Step 1}

Solve \ref{eq:FOClaborfinal}, \ref{eq:FOChardKfinal}, and \ref{eq:FOCsoftKfinal} for $k_i$, $\bar{k}_c = \frac{k_{c,1}}{h,1}$, and $\bar{k}_i = \frac{k_{i,1}}{h,1}$ in function of unknown wage $w$. It yields
\begin{equation}
\bar{k}_c = \frac{a}{1 - a- b}\frac{w}{r_c},
\end{equation}
\begin{equation}
\bar{k}_i = \frac{b}{1 - a- b}\frac{w}{r_i},
\end{equation}
and
\begin{equation}
k_i = \bigg[   \frac{r_c}{a \Gamma_c}   \bar{k}_c^{1-a} \bar{k}_i^{-b}   \bigg]^{\frac{1}{\gamma}}
\end{equation}
Moreover, divide \ref{eq:FOChardKfinal} over \ref{eq:FOCsoftKfinal} and obtain
\begin{equation}
\frac{\bar{k}_i}{\bar{k}_c} = \frac{b}{a} \frac{r_c}{r_i}
\end{equation}
Finally, using \ref{eq:FOClaborfinal}-\ref{eq:FOCsoftKinter} notice that 
$$
\bar{k}_c = \frac{k_{c,1}}{h_1} = \frac{k_{c,2}}{h_2} = \frac{k_{c}}{h},
$$
$$
\bar{k}_i = \frac{k_{i,1}}{h_1} = \frac{k_{i,2}}{h_2} = \frac{k_{i}}{h},
$$
and
$$
\frac{\bar{k}_i}{\bar{k}_c} = \frac{{k}_i}{{k}_c} = \frac{{k}_{i,1}}{{k}_{c,1}} = \frac{{k}_{i,2}}{{k}_{c,2}}.
$$

\subsection*{Step 2}

Obtain from \ref{eq:FOCsoftKinter}
\begin{equation}\label{eq:LOMinterSS}
i_i = G_i k_i 
\end{equation}
where $G_i = \exp(g_i) - (1 - \delta_i)$.

Substitute \ref{eq:LOMinterSS} into \ref{eq:resourceinter} and then into \ref{eq:prodfuncinter} to obtain
$$
G_i k_i = \Gamma_{i} k_{i}^{\gamma} h_{2}^{1 - a- b} k_{c,2}^a k_{i,2}^b
$$
which is
$$
G_i k_i = \Gamma_{i} k_{i}^{\gamma} h_{2} \bar{k}_{c,2}^a \bar{k}_{i,2}^b
$$
Isolate over $h_2$ and get
\begin{equation}
h_2 = \frac{G_i}{\Gamma_i} k_i^{1 - \gamma} \bar{k}_{c,2}^{-a} \bar{k}_{i,2}^{-b}
\end{equation}
which yields
$$
k_{i,2} = \bar{k}_i h_2 \ \ \text{and} \ \ k_{c,2} = \bar{k}_c h_2.
$$


\subsection*{Step 3}


Obtain from \ref{eq:FOCsoftKfinal}
\begin{equation}\label{eq:LOMfinalSS}
i_c = G_c k_c
\end{equation}
where $G_c = \exp(g_c) - (1 - \delta_c)$.

Substitute \ref{eq:LOMfinalSS} into \ref{eq:resourcefinal} and then into \ref{eq:prodfuncfinal} to obtain
$$
G_i k_i = \Gamma_{i} k_{i}^{\gamma} h_{2}^{1 - a- b} k_{c,2}^a k_{i,2}^b
$$
which is
$$
G_i k_i = \Gamma_{i} k_{i}^{\gamma} h_{2} \bar{k}_{c,2}^a \bar{k}_{i,2}^b
$$
Isolate over $h_2$ and get
\begin{equation}
h_2 = \frac{G_i}{\Gamma_i} k_i^{1 - \gamma} \bar{k}_{c,2}^{-a} \bar{k}_{i,2}^{-b}
\end{equation}
which yields
$$
k_{i,2} = \bar{k}_i h_2 \ \ \text{and} \ \ k_{c,2} = \bar{k}_c h_2.
$$


















\end{document}

